\documentclass{article}
\usepackage[margin=1in]{geometry}
\usepackage{amsmath}
\usepackage{amsthm}
\usepackage{amssymb}
\usepackage{graphicx}

\DeclareMathOperator*{\argmax}{arg\,max}
\DeclareMathOperator*{\argmin}{arg\,min}

\title{Assignment 12}
\author{Monte Fischer}

\begin{document}

\maketitle

\section*{Problem 2}

See the implementation in function \texttt{tabular\_td\_lambda} in \texttt{monte/assignment12/td\_lambda.py}.

\section*{Problem 3}

We wish to prove that the MC error is the sum of discounted TD errors:

\begin{equation}
    G_t - V(S_t) = \sum_{u=t}^{T-1} \gamma^{u-t} \cdot (R_{u+1} + \gamma \cdot V(S_{u+1}) - V(S_u))
\end{equation}

We proceed by backwards induction. Note that since
\begin{equation}
    G_t = R_{t+1} + \gamma R_{t+2} + \gamma^2 R_{t+3} + \dots + \gamma^{T-t-1} R_T
\end{equation}
we have
\begin{align*}
    G_{T-1} - V(S_{T-1}) &= R_T - V(S_{T-1}) \\
    &= \gamma^0 (R_T + \gamma V(S_T) - V(S_{T-1}))
\end{align*}
since $V(S_T) = 0$. Having established the above equality for $t=T-1$, we assume its truth for arbitrary $t + 1 > 0$ and show that it holds for $t$ as well. Calculating,

\begin{align}
    G_t - V_(S_t) &= R_{t+1} + \gamma G_{t+1} - V(S_t)\\
    &= \gamma (G_{t+1} - V(S_{t+1})) + R_{t+1} + \gamma V(S_{t+1}) - V(S_t)\\
    &= \gamma V(S_{t+1}) - V(S_t) + \sum_{u=t+1}^{T-1}\gamma^{u-t-1} (R_{u+1} + \gamma V(S_{u+1}) - V(S_u))\\
    &= \sum_{u=t}^{T-1} \gamma^{u-t} \cdot (R_{u+1} + \gamma \cdot V(S_{u+1}) - V(S_u)),
\end{align}
establishing the claim.

\end{document}
